erasure/theories/Prelim.v
@@ -392,7 +392,7 @@ Inductive red_decls Σ Γ Γ' : forall (x y : PCUICAst.context_decl), Type :=
   Σ ;;; Γ' |- b' : T -> red Σ Γ b b' ->
   red_decls Σ Γ Γ' (PCUICAst.vdef na b T) (PCUICAst.vdef na' b' T).
 
-Notation red_context Σ := (context_relation (red_decls Σ)).
+Notation red_context Σ := (All2_fold (red_decls Σ)).
 
 Lemma conv_context_app (Σ : global_env_ext) (Γ1 Γ2 Γ1' : context) :
   wf Σ ->
