pcuic/theories/PCUICSubstitution.v
@@ -364,7 +364,7 @@ Qed.
   subst_mutual_inductive_body n k decl = decl.
 Proof.
   intros wfΣ Hdecl.
-  pose proof (on_declared_minductive wfΣ Hdecl). apply onNpars in X.
+  pose proof (on_declsared_minductive wfΣ Hdecl). apply onNpars in X.
   apply (declared_inductive_closed (Σ:=(empty_ext Σ))) in Hdecl; auto.
   move: Hdecl.
   rewrite /closed_inductive_decl /lift_mutual_inductive_body.
@@ -1344,8 +1344,7 @@ Qed.
 Lemma subst_eq_decl `{checker_flags} {le Σ ϕ l k d d'} :
   eq_decl le Σ ϕ d d' -> eq_decl le Σ ϕ (subst_decl l k d) (subst_decl l k d').
 Proof.
-  destruct d, d', decl_body, decl_body0, le;
-    unfold eq_decl, map_decl; cbn; 
+  intros []; constructor; auto; destruct le; 
     intuition eauto using subst_compare_term, subst_eq_term, subst_leq_term.
 Qed.
 
@@ -1354,9 +1353,8 @@ Lemma subst_eq_context `{checker_flags} le Σ φ l l' n k :
   eq_context le Σ φ (subst_context n k l) (subst_context n k l').
 Proof.
   induction 1; rewrite ?subst_context_snoc /=; constructor; auto.
-  - erewrite (context_relation_length X). simpl.
-    apply (subst_eq_decl p).
-  - rewrite (context_relation_length X); simpl; apply (subst_eq_decl p).
+  erewrite (All2_fold_length X). simpl.
+  apply (subst_eq_decl p).
 Qed.
 
 Lemma substitution_red `{cf : checker_flags} (Σ : global_env_ext) Γ Δ Γ' s M N :
@@ -1369,8 +1367,7 @@ Proof.
   - etransitivity; eauto.
 Qed.
 
-(** With the new case representation, requires a well-formendness argument. 
-  But do we really need these untyped reduction lemmas? *)
+(** Do we really need these untyped reduction lemmas? *)
   
 Lemma red_red {cf:checker_flags} (Σ : global_env_ext) Γ Δ Γ' s s' b : wf Σ ->
   All2 (red Σ Γ) s s' ->
@@ -1712,7 +1709,7 @@ Proof.
     rewrite !map_cst_type. eapply subst_declared_constant in H as ->; eauto.
 
   - eapply refine_type. econstructor; eauto.
-    eapply on_declared_inductive in as isdecl [on_mind on_ind]; auto.
+    eapply on_declsared_inductive in as isdecl [on_mind on_ind]; auto.
     apply onArity in on_ind as [[s' Hindty] _].
     apply typecheck_closed in Hindty as [_ Hindty]; eauto. symmetry.
     move/andb_and/proj1: Hindty. rewrite -(closedn_subst_instance _ _ u) => Hty.
@@ -1721,7 +1718,7 @@ Proof.
 
   - eapply refine_type. econstructor; eauto.
     symmetry.
-    apply on_declared_constructor in isdecl as [_ onc]; auto.
+    apply on_declsared_constructor in isdecl as [_ onc]; auto.
     eapply on_constructor_closed in onc as clty; auto.
     unfold type_of_constructor.
     apply subst_closedn; eauto. eapply closed_upwards; eauto. lia.
@@ -1751,7 +1748,7 @@ Proof.
     erewrite distr_subst_rec. simpl.
     rewrite map_rev. subst ty.
     f_equal.
-    apply on_declared_projection in isdecl as [_ isdecl]; auto.
+    apply on_declsared_projection in isdecl as [_ isdecl]; auto.
     eapply on_projection_closed in isdecl as clty; auto.
     symmetry. apply subst_closedn; eauto.
     rewrite List.rev_length H. eapply closed_upwards; eauto. lia.
